



DH - Table (general)

i	a_i	α_i	d_i	θ_i
1	0	0	d_1	θ_1
2	0	$+90^\circ$	0	θ_2
3	a_3	0	0	θ_3
4	a_4	0	d_4	θ_4
5	0	-90°	d_5	θ_5
6	0	$+90^\circ$	d_6	θ_6

For the current Diagram Configuration - DH - Table is

i	a_i	α_i	d_i	θ_i
1	0	0	d_1	0
2	0	$+90^\circ$	0	0
3	a_3	0	0	90°
4	a_4	0	d_4	0
5	0	-90°	d_5	-90°
6	0	$+90^\circ$	d_6	0

(Vertically Fully Stretched case)

Transformation Matrix

$$T_i = R_z(\theta_i) T_z(d_i) T_x(a_i) R_x(\alpha_i) \rightarrow \text{Eq (1)}$$

Now,

Rotation about z:

$$R_z(\theta_i) = \begin{bmatrix} \cos \theta_i & -\sin \theta_i & 0 & 0 \\ \sin \theta_i & \cos \theta_i & 0 & 0 \\ 0 & 0 & 1 & 0 \\ 0 & 0 & 0 & 1 \end{bmatrix}$$

Translation along z:

$$T_z(d_i) = \begin{bmatrix} 1 & 0 & 0 & 0 \\ 0 & 1 & 0 & 0 \\ 0 & 0 & 1 & d_i \\ 0 & 0 & 0 & 1 \end{bmatrix}$$

Translation along x:

$$T_x(a_i) = \begin{bmatrix} 1 & 0 & 0 & a_i \\ 0 & 1 & 0 & 0 \\ 0 & 0 & 1 & 0 \\ 0 & 0 & 0 & 1 \end{bmatrix}$$

Rotation about x:

$$R_x(\alpha_i) = \begin{bmatrix} 1 & 0 & 0 & 0 \\ 0 & \cos \alpha_i & -\sin \alpha_i & 0 \\ 0 & \sin \alpha_i & \cos \alpha_i & 0 \\ 0 & 0 & 0 & 1 \end{bmatrix}$$

Now, after multiplying all the four like in Eqn 1, we get

$$T_i = \begin{bmatrix} \cos \theta_i & -\sin \theta_i \cos \alpha_i & \sin \theta_i \sin \alpha_i & a_i \cos \theta_i \\ \sin \theta_i & \cos \theta_i \cos \alpha_i & -\cos \theta_i \sin \alpha_i & a_i \sin \theta_i \\ 0 & \sin \alpha_i & \cos \alpha_i & d_i \\ 0 & 0 & 0 & 1 \end{bmatrix}$$

Example:

let

$$a_3 = a_4 = 1 \quad \& \quad d_1 = d_4 = d_5 = d_6 = 1$$

$$\& \quad \theta_i = [0^\circ, 0^\circ, 90^\circ, 0^\circ, -90^\circ, 0^\circ]$$

Mean vertically fully stretched case

$$\Rightarrow T_1 = \begin{bmatrix} 1 & 0 & 0 & 0 \\ 0 & 1 & 0 & 0 \\ 0 & 0 & 1 & 1 \\ 0 & 0 & 0 & 1 \end{bmatrix} \quad \text{since } a_1 = 0, \alpha_1 = 0, d_1 = 1, \theta_1 = 0$$

$$T_2 = \begin{bmatrix} 1 & 0 & 0 & 0 \\ 0 & 0 & -1 & 0 \\ 0 & 1 & 0 & 0 \\ 0 & 0 & 0 & 1 \end{bmatrix} \quad \text{since } a_2 = 0, \alpha_2 = \pi/2, d_2 = 0, \theta_2 = 0$$

$$T_3 = \begin{bmatrix} 0 & -1 & 0 & 0 \\ 1 & 0 & 0 & 1 \\ 0 & 0 & 1 & 0 \\ 0 & 0 & 0 & 1 \end{bmatrix} \quad \text{since } a_3 = 1, \alpha_3 = 0, d_3 = 0, \theta_3 = \pi/2$$

$$T_4 = \begin{bmatrix} 1 & 0 & 0 & 1 \\ 0 & 1 & 0 & 0 \\ 0 & 0 & 0 & 1 \\ 0 & 0 & 0 & 1 \end{bmatrix} \quad \text{since } a_4 = 1, \alpha_4 = 0, d_4 = 1, \theta_4 = 0$$

$$T_5 = \begin{bmatrix} 0 & 0 & 1 & 0 \\ -1 & 0 & 0 & 0 \\ 0 & -1 & 0 & 1 \\ 0 & 0 & 0 & 1 \end{bmatrix} \quad \text{since } a_5 = 0, \alpha_5 = -\pi/2, d_5 = 1, \theta_5 = -\pi/2$$

$$T_6 = \begin{bmatrix} 1 & 0 & 0 & 0 \\ 0 & 0 & -1 & 0 \\ 0 & 1 & 0 & 1 \\ 0 & 0 & 0 & 1 \end{bmatrix} \quad \text{since } a_6 = 0, \alpha_6 = \pi/2, d_6 = 1, \theta_6 = \pi/2$$

for transformation from some p to q ($p < q$)
index (Joint),

$$T_{pq} = T_{pa} T_{ab} T_{bc} T_{cd} \dots T_{-q}$$

where $p < a < b < \dots < q$
in joint index.

Similarly

$$T_{06} = T_{01} T_{12} T_{23} T_{34} T_{45} T_{56}$$

$$\Rightarrow T_{06} = \begin{bmatrix} 0 & 0 & 1 & 1 \\ 1 & 0 & 0 & 1 \\ 0 & 1 & 0 & 3 \\ 0 & 0 & 0 & 1 \end{bmatrix}$$

$$T_{06} = \begin{bmatrix} 1 & 0 & 0 & 0 \\ 0 & 0 & -1 & -2 \\ 0 & 1 & 0 & 4 \\ 0 & 0 & 0 & 1 \end{bmatrix}$$

from this

position of end-effector $p = \begin{bmatrix} 0 \\ -2 \\ 4 \end{bmatrix}$

$$\text{i.e. } (x, y, z) = (0, -2, 4)$$

$$\text{Rotation matrix is } R = \begin{bmatrix} 1 & 0 & 0 \\ 0 & 0 & -1 \\ 0 & 1 & 0 \end{bmatrix}$$

$$\Rightarrow \text{Roll} = 0^\circ, \text{pitch} = 0^\circ, \text{yaw} = 0^\circ$$

$$\det(R) = 1,$$

Jacobian column/Matrix

for revolute joint

$$J_{v,i} = z_{i-1} \times (O_n - O_{i-1})$$

$$J_{w,i} = z_{i-1}$$

for Joint 1

1)

$$z_0 = \begin{bmatrix} 0 \\ 0 \\ 1 \end{bmatrix} ; O_n = \begin{bmatrix} x \\ y \\ z \end{bmatrix} \rightarrow \text{end-effector} \quad \text{or } O_0 = \begin{bmatrix} 0 \\ 0 \\ 0 \end{bmatrix} \quad \text{origin of frame 0}$$

$$\Rightarrow J_{v,1} = \begin{bmatrix} 0 \\ 0 \\ 1 \end{bmatrix} \times \left(\begin{bmatrix} x \\ y \\ z \end{bmatrix} - \begin{bmatrix} 0 \\ 0 \\ 0 \end{bmatrix} \right)$$

$$\therefore J_{v,1} = \begin{bmatrix} -y \\ x \\ 0 \end{bmatrix}$$

$$\text{Now, } J_{w,1} = \begin{bmatrix} 0 \\ 0 \\ 1 \end{bmatrix}$$

$$\Rightarrow J_1 = \begin{bmatrix} \begin{bmatrix} -y \\ x \\ 0 \end{bmatrix} \\ \begin{bmatrix} 0 \\ 0 \\ 1 \end{bmatrix} \end{bmatrix} \begin{matrix} \rightarrow J_{v,1} \\ \rightarrow J_{w,1} \end{matrix}$$

similarly we have to do for all joints then the Jacobian matrix be

$$J = \begin{bmatrix} [J_1] & [J_2] & [J_3] & [J_4] & [J_5] & [J_6] \end{bmatrix}_{6 \times 6}$$

Example:

again let $a_3 = a_4 = 1$; $d_1 = d_4 = d_5 = d_6 = 1$

$$\theta_i = [0^\circ, 0^\circ, 90^\circ, 0^\circ, -90^\circ, 0^\circ]$$

from result in Transformation Example,

$$T_{06} = \begin{bmatrix} 1 & 0 & 0 & 0 \\ 0 & 0 & -1 & -2 \\ 0 & 1 & 0 & 4 \\ 0 & 0 & 0 & 1 \end{bmatrix}$$

$$\Rightarrow O_6 = \begin{bmatrix} 0 \\ -2 \\ 4 \end{bmatrix}$$

In Joint

$$1) \quad z_0 = \begin{bmatrix} 0 \\ 0 \\ 1 \end{bmatrix} \quad \text{or } O_0 = \begin{bmatrix} 0 \\ 0 \\ 0 \end{bmatrix}$$

$$\Rightarrow J_{v11} = \begin{bmatrix} 0 \\ 0 \\ 1 \end{bmatrix} \times \left(\begin{bmatrix} 0 \\ -2 \\ 4 \end{bmatrix} - \begin{bmatrix} 0 \\ 0 \\ 0 \end{bmatrix} \right)$$

$$\Rightarrow J_{v11} = \begin{bmatrix} 2 \\ 0 \\ 0 \end{bmatrix}$$

$$J_{w11} = \begin{bmatrix} 0 \\ 0 \\ 1 \end{bmatrix}$$

$$\Rightarrow J_1 = \begin{bmatrix} 2 \\ 0 \\ 0 \\ 0 \\ 0 \\ 1 \end{bmatrix}$$

2)

$$z_1 = \begin{bmatrix} 0 \\ 0 \\ 1 \end{bmatrix}$$

$$O_1 = [0, 0, 1]^T$$

Since ~~z_1 is same as z_2~~

$$J_1 = J_2$$

$$\Rightarrow J_2 = \begin{bmatrix} 2 \\ 0 \\ 0 \\ 0 \\ 0 \\ 1 \end{bmatrix}$$

3)

$$z_2 = \begin{bmatrix} 0 \\ -1 \\ 0 \end{bmatrix} \propto O = \begin{bmatrix} 0 \\ 0 \\ 1 \end{bmatrix}$$

$$J_{03} = \begin{bmatrix} 0 \\ 1 \\ 0 \end{bmatrix} \times \left(\begin{bmatrix} 0 \\ -2 \\ 4 \end{bmatrix} - \begin{bmatrix} 0 \\ 0 \\ 1 \end{bmatrix} \right)$$

$$J_{03} = \begin{bmatrix} 3 \\ 0 \\ 0 \\ 0 \\ 1 \\ 0 \end{bmatrix}$$

Similarly we get all J_i upto J_6 from J_1

at last we will get

$$J = \begin{pmatrix} 2 & 2 & -3 & -2 & -1 & 0 \\ 0 & 0 & 0 & 0 & 0 & 0 \\ 0 & 0 & 0 & 0 & 0 & 0 \\ 0 & 0 & 0 & 0 & 0 & 0 \\ 0 & 0 & -1 & -1 & -1 & 0 \\ 1 & 1 & 0 & 0 & 0 & 1 \end{pmatrix}$$

∴

$$\det(J) = 0$$

→ Robot is in a singular configuration!